@prefix rdfs:  <http://www.w3.org/2000/01/rdf-schema#> .
@prefix xsd:   <http://www.w3.org/2001/XMLSchema#> .
@prefix owl:   <http://www.w3.org/2002/07/owl#> .
@prefix rdf:   <http://www.w3.org/1999/02/22-rdf-syntax-ns#> .

@prefix li:    <http://www.epimorphics.com/public/vocabulary/lucene-index#> .
@prefix :      <http://www.epimorphics.com/public/vocabulary/lucene-index#> .

:Config a owl:Class;
    rdfs:label "Config"@en;
    rdfs:comment "A configuration specification for a lucene based entity index"@en;
    .

:labelProp a owl:ObjectProperty;
    rdfs:label "label prop"@en;
    rdfs:comment "Indicates a property whose values should be parsed as free text and indexed and stored."@en;
    rdfs:domain :Config;
    rdfs:range  rdf:property;
    .

:labelOnlyProp a owl:ObjectProperty;
    rdfs:label "label only prop"@en;
    rdfs:comment "Indicates a property whose values should be parsed as free text and indexed, but not stored."@en;
    rdfs:domain :Config;
    rdfs:range  rdf:property;
    .

:valueProp a owl:ObjectProperty;
    rdfs:label "value prop"@en;
    rdfs:comment "Indicates a property whose values should be indexed as a simple value node and stored."@en;
    rdfs:domain :Config;
    rdfs:range  rdf:property;
    .

:ignoreProp a owl:ObjectProperty;
    rdfs:label "ignore prop"@en;
    rdfs:comment "Indicates a property whose values should be ignored for indexing."@en;
    rdfs:domain :Config;
    rdfs:range  rdf:property;
    .

:categoryProp a owl:ObjectProperty;
    rdfs:label "category prop"@en;
    rdfs:comment "Indicates a property whose value should be added to a faceted browse taxonomy index."@en;
    rdfs:domain :Config;
    rdfs:range  rdf:property;
    .

:conceptScheme a owl:ObjectProperty;
    rdfs:label "concept scheme"@en;
    rdfs:comment "Indicates a skos:ConceptScheme which provides a hiearchical structure for category prop indexing."@en;
    rdfs:domain :Config;
    rdfs:range  rdf:property;
    .

:indexAll a owl:ObjectProperty;
    rdfs:label "label prop"@en;
    rdfs:comment "If true then all properties on the entity which aren't explicitly ingored or already indexed should be indexed as simple values."@en;
    rdfs:domain :Config;
    rdfs:range  xsd:boolean;
    .

    
